fix spec

specs/experimental/rsapss/Spec.RSA.Lemmas.fst
@@ -53,29 +53,17 @@ val lemma_pow_mul:
   (pow (a * b) c = (pow a c) * (pow b c))
 let lemma_pow_mul a b c = admit()
 
-val lemma_pow_div:
-  a:nat -> b:nat -> d:nat{d > 0} -> Lemma
-  (pow (a / d) b = (pow a b) / pow d b)
-let lemma_pow_div a b d = admit()
-
-val lemma_pow_a2_b:
-  a:nat -> b:nat -> Lemma
-  (pow (a * a) b = pow a (2 * b))
-let lemma_pow_a2_b a b =
-  lemma_pow_mul a a b;
-  lemma_pow a b b
-
 val lemma_pow_mod:
   a:nat -> b:nat -> n:pos -> Lemma
   ((pow a b) % n == (pow (a % n) b) % n)
 let lemma_pow_mod a b n = admit()
 
+// (1 / d) % n is an inverse element of d
 val lemma_mod_mult_div_1:
   a:nat -> d:nat{d > 0} -> n:nat{n > 0} -> Lemma
   ((a / d) % n == ((a % n) / d) % n)
 let lemma_mod_mult_div_1 a d n = admit()
 
-// (1 / d) % n is an inverse element of d
 val lemma_mod_mult_div:
   a:nat -> b:nat -> d:nat{d > 0} -> n:nat{n > 0} -> Lemma
   ((a * b / d) % n == ((a % n) * b / d) % n)
@@ -151,11 +139,8 @@ val lemma_get_bit_first:
 let lemma_get_bit_first bBits b i =
   let c = bn_v b % pow2 (i+1) in
   euclidean_division_definition c (pow2 i);
-  //assert (c == c % pow2 i + pow2 i * (c / pow2 i));
   pow2_modulo_modulo_lemma_1 (bn_v b) i (i+1);
-  //assert (c == bn_v b % pow2 i + pow2 i * (c / pow2 i));
   pow2_modulo_division_lemma_1 (bn_v b) i (i+1)
-  //assert (c == bn_v b % pow2 i + pow2 i * ((bn_v b / pow2 i) % 2))
 
 val mod_exp_pred:
   nBits:size_pos ->
@@ -194,12 +179,9 @@ let lemma_mod_exp_f1 nBits rBits nInv_u64 n bBits b a0 acc0 a acc a1 i =
      assert_norm (bn_v (bn_get_bits_first b i) == 0);
      assert_norm (pow (bn_v a0) (bn_v (bn_get_bits_first b (i+1))) == 1);
      assert_norm (pow (pow2 rBits) (bn_v (bn_get_bits_first b (i+1))) == 1);
-     //assert_norm (bn_v acc % bn_v n == ((pow (bn_v a0) (bn_v (bn_get_bits_first b (i+1))) * bn_v acc0) / pow (pow2 rBits) (bn_v (bn_get_bits_first b (i+1)))) % bn_v n);
      assert (mod_exp_pred nBits rBits nInv_u64 n bBits b a0 acc0 (i+1) (a1, acc)) end
   else begin
      assert (bn_v acc % bn_v n = ((pow (bn_v a0) (bn_v (bn_get_bits_first b i)) * bn_v acc0) / pow (pow2 rBits) (bn_v (bn_get_bits_first b i))) % bn_v n);
-     //assert_norm (pow (bn_v a0) (bn_v (bn_get_bits_first b (i+1))) == pow (bn_v a0) (bn_v (bn_get_bits_first b i)));
-     //assert_norm (pow (pow2 rBits) (bn_v (bn_get_bits_first b (i+1))) == pow (pow2 rBits) (bn_v (bn_get_bits_first b i)));
      assert (mod_exp_pred nBits rBits nInv_u64 n bBits b a0 acc0 (i+1) (a1, acc))
   end
 
@@ -222,8 +204,6 @@ val lemma_mod_exp_f20:
   (ensures (mod_exp_pred nBits rBits nInv_u64 n bBits b a0 acc0 (i+1) (a1, acc1)))
   #reset-options "--z3rlimit 150 --max_fuel 0"
 let lemma_mod_exp_f20 nBits rBits nInv_u64 n bBits b a0 acc0 a acc a1 acc1 i =
-  assert (bn_v acc % bn_v n == ((pow (bn_v a0) (bn_v (bn_get_bits_first b i)) * bn_v acc0) / pow (pow2 rBits) (bn_v (bn_get_bits_first b i))) % bn_v n);
-  assert (bn_v a % bn_v n == (pow (bn_v a0) (pow2 i) / pow (pow2 rBits) (pow2 i - 1)) % bn_v n);
   assert (bn_v acc1 % bn_v n == ((bn_v a * bn_v acc) / pow2 rBits) % bn_v n);
   lemma_mod_mult_div_1 (bn_v a * bn_v acc) (pow2 rBits) (bn_v n);
   lemma_mod_plus_mul_distr 0 (bn_v a) (bn_v acc) (bn_v n);
@@ -239,18 +219,13 @@ let lemma_mod_exp_f20 nBits rBits nInv_u64 n bBits b a0 acc0 a acc a1 acc1 i =
   lemma_mul_div_mod al bl cl dl (pow2 rBits) (bn_v n);
   assert (bn_v acc1 % bn_v n == ((al * cl) / (bl * dl * pow2 rBits)) % bn_v n);
   lemma_get_bit_first bBits b i;
-  //assert (bn_v (bn_get_bits_first b (i+1)) == bn_v (bn_get_bits_first b i) + pow2 i * bn_get_bit b i);
-  assert (bn_v (bn_get_bits_first b (i+1)) == bn_v (bn_get_bits_first b i) + pow2 i);
   lemma_pow (bn_v a0) (pow2 i) (bn_v (bn_get_bits_first b i));
   assert (al * cl == pow (bn_v a0) (bn_v (bn_get_bits_first b (i+1))) * bn_v acc0);
   lemma_pow (pow2 rBits) (pow2 i - 1) 1;
   assert_norm (pow2 rBits == pow (pow2 rBits) 1);
-  //assert (bl * pow2 rBits == pow (pow2 rBits) (pow2 i));
   lemma_pow (pow2 rBits) (pow2 i) (bn_v (bn_get_bits_first b i));
   lemma_mul_mul  bl dl (pow2 rBits);
-  //assert (bl * dl * pow2 rBits == bl * pow2 rBits * dl);
-  assert (bl * dl * pow2 rBits == pow (pow2 rBits) (bn_v (bn_get_bits_first b (i+1))));
-  assert (mod_exp_pred nBits rBits nInv_u64 n bBits b a0 acc0 (i+1) (a1, acc1))
+  assert (bl * dl * pow2 rBits == pow (pow2 rBits) (bn_v (bn_get_bits_first b (i+1))))
 
 val lemma_mod_exp_f2:
   nBits:size_pos -> rBits:size_pos{nBits + 2 < rBits /\ nBits + rBits + 1 < max_size_t /\ rBits % 64 == 0} ->
@@ -354,161 +329,6 @@ let lemma_mod_exp_2 n a a_r b acc_r r res_r =
   lemma_mod_mul_distr_l acc_r (pow a b) n;
   lemma_mod_mul_distr_l r (pow a b) n
 
-(* LEMMAS for exponent blinding *)
-let elem n = x:nat{x < n}
-
-val lemma_mod_pq:
-  a:nat -> b:nat -> p:nat{p > 1} -> q:nat{q > 1} -> Lemma
-  (requires (a % p == b % p /\ a % q == b % q))
-  (ensures (a % (p * q) == b % (p * q)))
-let lemma_mod_pq a b p q = admit()
-
-// m ^ (p - 1) = 1 (mod p) where gcd(m, p) = 1 and p is a prime number
-val fermat_little_theorem:
-  p:nat{p > 1} -> m:nat{m > 0} -> Lemma
-  (requires (m % p <> 0))
-  (ensures ((pow m (p - 1)) % p == 1))
-let fermat_little_theorem p m = admit()
-
-val lemma_exp_blinding_q:
-  n:nat{n > 0} -> phi_n:nat -> p:elem n{p > 0} ->
-  q:elem n{q > 0} -> m:elem n{m > 0} -> Lemma
-  (requires (phi_n == (p - 1) * (q - 1) /\ n = p * q /\ m % q <> 0))
-  (ensures ((pow m phi_n) % q == 1))
-  #reset-options "--z3rlimit 50 --max_fuel 0"
-let lemma_exp_blinding_q n phi_n p q m =
-  let res = (pow m phi_n) % q in
-  lemma_pow_pow m (q - 1) (p - 1);
-  lemma_pow_mod (pow m (q - 1)) (p - 1) q;
-  fermat_little_theorem q m;
-  lemma_pow_1 (p - 1)
-
-val lemma_exp_blinding_pq:
-  n:nat{n > 0} -> phi_n:nat -> p:elem n{p > 0} ->
-  q:elem n{q > 0} -> m:elem n{m > 0} -> Lemma
-  (requires (phi_n == (p - 1) * (q - 1) /\ n = p * q /\ m % p <> 0 /\ m % q <> 0))
-  (ensures ((pow m phi_n) % (p * q) == 1))
-  #reset-options "--z3rlimit 50 --max_fuel 0"
-let lemma_exp_blinding_pq n phi_n p q m =
-  lemma_exp_blinding_q n phi_n p q m;
-  small_modulo_lemma_1 1 q;
-  lemma_exp_blinding_q n phi_n q p m;
-  small_modulo_lemma_1 1 p;
-  lemma_mod_pq (pow m phi_n) 1 p q;
-  small_modulo_lemma_1 1 n
-
-val lemma_exp_blinding_1:
-  n:nat{n > 0} -> phi_n:nat -> p:elem n{p > 0} -> q:elem n{q > 0} ->
-  d:elem n{d > 0} -> m:elem n{m > 0} -> r:nat -> Lemma
-  (requires (phi_n = (p - 1) * (q - 1) /\ n = p * q /\ m % p <> 0 /\ m % q <> 0))
-  (ensures ((pow m (d + r * phi_n)) % n  == (pow m d) % n))
-let lemma_exp_blinding_1 n phi_n p q d m r =
-  lemma_exp_blinding_pq n phi_n p q m;
-  assert ((pow m phi_n) % (p * q) == 1);
-  let res:nat = (pow m (d + r * phi_n)) % n in
-  lemma_pow m d (r * phi_n);
-  lemma_pow_pow m phi_n r;
-  lemma_pow_mod (pow m phi_n) r n;
-  assert ((pow (pow m phi_n) r) % n == (pow ((pow m phi_n) % n) r) % n);
-  //assert ((pow (pow m phi_n) r) % n == (pow 1 r) % n);
-  lemma_pow_1 r;
-  modulo_lemma 1 n;
-  lemma_mod_mul_distr_l (pow m (r * phi_n)) (pow m d) n
-
-val lemma_exp_blinding_0_q0:
-  n:nat{n > 0} -> phi_n:nat -> p:elem n{p > 0} -> q:elem n{q > 0} ->
-  d:elem n{d > 0} -> m:elem n{m > 0} -> r:nat -> Lemma
-  (requires (phi_n = (p - 1) * (q - 1) /\ n = p * q /\ m % q = 0))
-  (ensures ((pow m (d + r * phi_n)) % q == (pow m d) % q))
-let lemma_exp_blinding_0_q0 n phi_n p q d m r =
-  let res:nat = pow m (d + r * phi_n) in
-  assert (res % q == (pow m (d + r * phi_n)) % q);
-  lemma_pow_mod m (d + r * phi_n) q;
-  lemma_pow_0 (d + r * phi_n);
-  lemma_pow_mod m d q;
-  lemma_pow_0 d
-
-val lemma_exp_blinding_0_q1:
-  n:nat{n > 0} -> phi_n:nat -> p:elem n{p > 0} -> q:elem n{q > 0} ->
-  d:elem n{d > 0} -> m:elem n{m > 0} -> r:nat -> Lemma
-  (requires (phi_n = (p - 1) * (q - 1) /\ n = p * q /\ m % p <> 0))
-  (ensures ((pow m (d + r * phi_n)) % p == (pow m d) % p))
-let lemma_exp_blinding_0_q1 n phi_n p q d m r =
-  lemma_exp_blinding_q n phi_n q p m;
-  assert ((pow m phi_n) % p == 1);
-  let res:nat = pow m (d + r * phi_n) in
-  assert (res % p == (pow m (d + r * phi_n)) % p);
-  lemma_pow m d (r * phi_n);
-  assert (res % p == ((pow m d) * (pow m (r * phi_n))) % p);
-  lemma_mod_mul_distr_l (pow m (r * phi_n)) (pow m d) p;
-  lemma_pow_pow m phi_n r;
-  lemma_pow_mod (pow m phi_n) r p;
-  assert ((pow m (r * phi_n)) % p == (pow ((pow m phi_n) % p) r) % p);
-  assert ((pow (pow m phi_n) r) % p == (pow 1 r) % p);
-  lemma_pow_1 r;
-  modulo_lemma 1 p;
-  assert (res % p == ((pow m d) * 1) % p)
-
-val lemma_exp_blinding_0_q:
-  n:nat{n > 0} -> phi_n:nat -> p:elem n{p > 0} -> q:elem n{q > 0} ->
-  d:elem n{d > 0} -> m:elem n{m > 0} -> r:nat -> Lemma
-  (requires (phi_n = (p - 1) * (q - 1) /\ n = p * q /\ m % q = 0 /\ m % p <> 0))
-  (ensures ((pow m (d + r * phi_n)) % n == (pow m d) % n))
-let lemma_exp_blinding_0_q n phi_n p q d m r =
-  let res:nat = pow m (d + r * phi_n) in
-  lemma_exp_blinding_0_q0 n phi_n p q d m r;
-  lemma_exp_blinding_0_q1 n phi_n p q d m r;
-  lemma_mod_pq res (pow m d) p q;
-  assert (res % n == (pow m d) % n)
-
-val lemma_exp_blinding_0_pq:
-  n:nat{n > 0} -> phi_n:nat -> p:elem n{p > 0} -> q:elem n{q > 0} ->
-  d:elem n{d > 0} -> m:elem n -> r:nat -> Lemma
-  (requires (phi_n = (p - 1) * (q - 1) /\ n = p * q /\ m % q = 0 /\ m % p = 0))
-  (ensures ((pow m (d + r * phi_n)) % n == (pow m d) % n))
-let lemma_exp_blinding_0_pq n phi_n p q d m r =
-  small_modulo_lemma_1 0 p;
-  small_modulo_lemma_1 0 q;
-  lemma_mod_pq m 0 p q;
-  small_modulo_lemma_1 0 n;
-  assert (m % n == 0);
-  small_modulo_lemma_1 m n;
-  assert (m = 0);
-  lemma_pow_0 (d + r * phi_n);
-  lemma_pow_0 d
-
-val lemma_exp_blinding_0:
-  n:nat{n > 0} -> phi_n:nat -> p:elem n{p > 0} -> q:elem n{q > 0} ->
-  d:elem n{d > 0} -> m:elem n -> r:nat -> Lemma
-  (requires (phi_n = (p - 1) * (q - 1) /\ n = p * q /\
-            (m = 0 \/ m % p = 0 \/ m % q = 0)))
-  (ensures ((pow m (d + r * phi_n)) % n  == (pow m d) % n))
-let lemma_exp_blinding_0 n phi_n p q d m r =
-  if (m = 0) then begin
-    lemma_pow_0 (d + r * phi_n);
-    lemma_pow_0 d end
-  else begin
-    if (m % p = 0 && m % q <> 0) then
-      lemma_exp_blinding_0_q n phi_n q p d m r
-    else begin
-      if (m % q = 0 && m % p <> 0) then
-	lemma_exp_blinding_0_q n phi_n p q d m r
-      else begin
-	assert (m % p = 0 && m % q = 0);
-	lemma_exp_blinding_0_pq n phi_n p q d m r end
-    end
-  end
-
-val lemma_exp_blinding:
-  n:nat{n > 0} -> phi_n:nat -> p:elem n{p > 0} -> q:elem n{q > 0} ->
-  d:elem n{d > 0} -> m:elem n -> r:nat -> Lemma
-  (requires (phi_n = (p - 1) * (q - 1) /\ n = p * q))
-  (ensures ((pow m (d + r * phi_n)) % n  == (pow m d) % n))
-let lemma_exp_blinding n phi_n p q d m r =
-  if (m = 0 || m % p = 0 || m % q = 0) then
-    lemma_exp_blinding_0 n phi_n p q d m r
-  else lemma_exp_blinding_1 n phi_n p q d m r
-
 (* LEMMAS for Karatsuba's multiplication *)
 val abs: x:int -> Tot (y:nat{(x >= 0 ==> y = x) /\ (x < 0 ==> y = -x)})
 let abs x = if x >= 0 then x else -x
@@ -517,6 +337,16 @@ val lemma_distributivity_mult:
   a:nat -> b:nat -> c:nat -> d:nat -> Lemma
   ((a + b) * (c + d) = a * c + a * d + b * c + b * d)
 let lemma_distributivity_mult a b c d = ()
+
+val lemma_add_sign1:
+  a0Bits:size_pos -> a1Bits:size_pos{a0Bits + a1Bits + 1 < max_size_t} ->
+  a0:bignum a0Bits -> a1:bignum a1Bits ->
+  b0:bignum a0Bits -> b1:bignum a1Bits -> Lemma
+  (bn_v a1 * bn_v b0 + bn_v a0 * bn_v b1 < pow2 (a0Bits + a1Bits + 1))
+let lemma_add_sign1 a0Bits a1Bits a0 a1 b0 b1 =
+  assert (bn_v a1 * bn_v b0 + bn_v a0 * bn_v b1 < pow2 a1Bits * pow2 a0Bits + pow2 a0Bits * pow2 a1Bits);
+  pow2_plus a1Bits a0Bits;
+  pow2_double_sum (a0Bits + a1Bits)
 
 val lemma_karatsuba_mult:
   aBits:size_pos -> a0Bits:size_pos -> a1Bits:size_pos{a0Bits + a1Bits == aBits} ->
@@ -552,12 +382,169 @@ let lemma_get_bits aBits a0Bits a a0 a1 =
   assert (bn_v a1 == bn_v a / pow2 a0Bits);
   euclidean_division_definition (bn_v a) (pow2 a0Bits)
 
-val lemma_add_sign1:
-  a0Bits:size_pos -> a1Bits:size_pos{a0Bits + a1Bits + 1 < max_size_t} ->
-  a0:bignum a0Bits -> a1:bignum a1Bits ->
-  b0:bignum a0Bits -> b1:bignum a1Bits -> Lemma
-  (bn_v a1 * bn_v b0 + bn_v a0 * bn_v b1 < pow2 (a0Bits + a1Bits + 1))
-let lemma_add_sign1 a0Bits a1Bits a0 a1 b0 b1 =
-  assert (bn_v a1 * bn_v b0 + bn_v a0 * bn_v b1 < pow2 a1Bits * pow2 a0Bits + pow2 a0Bits * pow2 a1Bits);
-  pow2_plus a1Bits a0Bits;
-  pow2_double_sum (a0Bits + a1Bits)
+(* LEMMAS for exponent blinding *)
+let elem n = x:nat{x < n}
+
+val lemma_mod_pq:
+  a:nat -> b:nat -> p:nat{p > 1} -> q:nat{q > 1} -> Lemma
+  (requires (a % p == b % p /\ a % q == b % q))
+  (ensures (a % (p * q) == b % (p * q)))
+let lemma_mod_pq a b p q = admit()
+
+// m ^ (p - 1) = 1 (mod p) where gcd(m, p) = 1 and p is a prime number
+val fermat_little_theorem:
+  p:nat{p > 1} -> m:nat{m > 0} -> Lemma
+  (requires (m % p <> 0))
+  (ensures ((pow m (p - 1)) % p == 1))
+let fermat_little_theorem p m = admit()
+
+val lemma_exp_blinding_q:
+  n:nat{n > 1} -> phi_n:nat -> p:elem n{p > 1} ->
+  q:elem n{q > 1} -> m:elem n{m > 0} -> Lemma
+  (requires (phi_n == (p - 1) * (q - 1) /\ n = p * q /\ m % q <> 0))
+  (ensures ((pow m phi_n) % q == 1))
+  #reset-options "--z3rlimit 50 --max_fuel 0"
+let lemma_exp_blinding_q n phi_n p q m =
+  let res = (pow m phi_n) % q in
+  lemma_pow_pow m (q - 1) (p - 1);
+  lemma_pow_mod (pow m (q - 1)) (p - 1) q;
+  fermat_little_theorem q m;
+  lemma_pow_1 (p - 1)
+
+val lemma_exp_blinding_pq:
+  n:nat{n > 1} -> phi_n:nat -> p:elem n{p > 1} ->
+  q:elem n{q > 1} -> m:elem n{m > 0} -> Lemma
+  (requires (phi_n == (p - 1) * (q - 1) /\ n = p * q /\ m % p <> 0 /\ m % q <> 0))
+  (ensures ((pow m phi_n) % (p * q) == 1))
+  #reset-options "--z3rlimit 50 --max_fuel 0"
+let lemma_exp_blinding_pq n phi_n p q m =
+  lemma_exp_blinding_q n phi_n p q m;
+  small_modulo_lemma_1 1 q;
+  lemma_exp_blinding_q n phi_n q p m;
+  small_modulo_lemma_1 1 p;
+  lemma_mod_pq (pow m phi_n) 1 p q;
+  small_modulo_lemma_1 1 n
+
+val lemma_exp_blinding_1:
+  n:nat{n > 1} -> phi_n:nat -> p:elem n{p > 1} -> q:elem n{q > 1} ->
+  d:elem n{d > 0} -> m:elem n{m > 0} -> r:nat -> Lemma
+  (requires (phi_n = (p - 1) * (q - 1) /\ n = p * q /\ m % p <> 0 /\ m % q <> 0))
+  (ensures ((pow m (d + r * phi_n)) % n  == (pow m d) % n))
+let lemma_exp_blinding_1 n phi_n p q d m r =
+  lemma_exp_blinding_pq n phi_n p q m;
+  assert ((pow m phi_n) % (p * q) == 1);
+  let res:nat = (pow m (d + r * phi_n)) % n in
+  lemma_pow m d (r * phi_n);
+  lemma_pow_pow m phi_n r;
+  lemma_pow_mod (pow m phi_n) r n;
+  assert ((pow (pow m phi_n) r) % n == (pow ((pow m phi_n) % n) r) % n);
+  //assert ((pow (pow m phi_n) r) % n == (pow 1 r) % n);
+  lemma_pow_1 r;
+  modulo_lemma 1 n;
+  lemma_mod_mul_distr_l (pow m (r * phi_n)) (pow m d) n
+
+val lemma_exp_blinding_0_q0:
+  n:nat{n > 1} -> phi_n:nat -> p:elem n{p > 1} -> q:elem n{q > 1} ->
+  d:elem n{d > 0} -> m:elem n{m > 0} -> r:nat -> Lemma
+  (requires (phi_n = (p - 1) * (q - 1) /\ n = p * q /\ m % q = 0))
+  (ensures ((pow m (d + r * phi_n)) % q == (pow m d) % q))
+let lemma_exp_blinding_0_q0 n phi_n p q d m r =
+  let res:nat = pow m (d + r * phi_n) in
+  assert (res % q == (pow m (d + r * phi_n)) % q);
+  lemma_pow_mod m (d + r * phi_n) q;
+  lemma_pow_0 (d + r * phi_n);
+  lemma_pow_mod m d q;
+  lemma_pow_0 d
+
+val lemma_exp_blinding_0_q1:
+  n:nat{n > 1} -> phi_n:nat -> p:elem n{p > 1} -> q:elem n{q > 1} ->
+  d:elem n{d > 0} -> m:elem n{m > 0} -> r:nat -> Lemma
+  (requires (phi_n = (p - 1) * (q - 1) /\ n = p * q /\ m % p <> 0))
+  (ensures ((pow m (d + r * phi_n)) % p == (pow m d) % p))
+let lemma_exp_blinding_0_q1 n phi_n p q d m r =
+  lemma_exp_blinding_q n phi_n q p m;
+  assert ((pow m phi_n) % p == 1);
+  let res:nat = pow m (d + r * phi_n) in
+  assert (res % p == (pow m (d + r * phi_n)) % p);
+  lemma_pow m d (r * phi_n);
+  assert (res % p == ((pow m d) * (pow m (r * phi_n))) % p);
+  lemma_mod_mul_distr_l (pow m (r * phi_n)) (pow m d) p;
+  lemma_pow_pow m phi_n r;
+  lemma_pow_mod (pow m phi_n) r p;
+  assert ((pow m (r * phi_n)) % p == (pow ((pow m phi_n) % p) r) % p);
+  assert ((pow (pow m phi_n) r) % p == (pow 1 r) % p);
+  lemma_pow_1 r;
+  modulo_lemma 1 p;
+  assert (res % p == ((pow m d) * 1) % p)
+
+val lemma_exp_blinding_0_q:
+  n:nat{n > 1} -> phi_n:nat -> p:elem n{p > 1} -> q:elem n{q > 1} ->
+  d:elem n{d > 0} -> m:elem n{m > 0} -> r:nat -> Lemma
+  (requires (phi_n = (p - 1) * (q - 1) /\ n = p * q /\ m % q = 0 /\ m % p <> 0))
+  (ensures ((pow m (d + r * phi_n)) % n == (pow m d) % n))
+let lemma_exp_blinding_0_q n phi_n p q d m r =
+  let res:nat = pow m (d + r * phi_n) in
+  lemma_exp_blinding_0_q0 n phi_n p q d m r;
+  lemma_exp_blinding_0_q1 n phi_n p q d m r;
+  lemma_mod_pq res (pow m d) p q;
+  assert (res % n == (pow m d) % n)
+
+val lemma_exp_blinding_0_pq:
+  n:nat{n > 1} -> phi_n:nat -> p:elem n{p > 1} -> q:elem n{q > 1} ->
+  d:elem n{d > 0} -> m:elem n -> r:nat -> Lemma
+  (requires (phi_n = (p - 1) * (q - 1) /\ n = p * q /\ m % q = 0 /\ m % p = 0))
+  (ensures ((pow m (d + r * phi_n)) % n == (pow m d) % n))
+let lemma_exp_blinding_0_pq n phi_n p q d m r =
+  small_modulo_lemma_1 0 p;
+  small_modulo_lemma_1 0 q;
+  lemma_mod_pq m 0 p q;
+  small_modulo_lemma_1 0 n;
+  assert (m % n == 0);
+  small_modulo_lemma_1 m n;
+  assert (m = 0);
+  lemma_pow_0 (d + r * phi_n);
+  lemma_pow_0 d
+
+val lemma_exp_blinding_0:
+  n:nat{n > 1} -> phi_n:nat -> p:elem n{p > 1} -> q:elem n{q > 1} ->
+  d:elem n{d > 0} -> m:elem n -> r:nat -> Lemma
+  (requires (phi_n = (p - 1) * (q - 1) /\ n = p * q /\
+            (m = 0 \/ m % p = 0 \/ m % q = 0)))
+  (ensures ((pow m (d + r * phi_n)) % n  == (pow m d) % n))
+let lemma_exp_blinding_0 n phi_n p q d m r =
+  if (m = 0) then begin
+    lemma_pow_0 (d + r * phi_n);
+    lemma_pow_0 d end
+  else begin
+    if (m % p = 0 && m % q <> 0) then
+      lemma_exp_blinding_0_q n phi_n q p d m r
+    else begin
+      if (m % q = 0 && m % p <> 0) then
+	lemma_exp_blinding_0_q n phi_n p q d m r
+      else begin
+	assert (m % p = 0 && m % q = 0);
+	lemma_exp_blinding_0_pq n phi_n p q d m r end
+    end
+  end
+
+val lemma_exp_blinding:
+  n:nat{n > 1} -> phi_n:nat -> p:elem n{p > 1} -> q:elem n{q > 1} ->
+  d:elem n{d > 0} -> m:elem n -> r:nat -> Lemma
+  (requires (phi_n = (p - 1) * (q - 1) /\ n = p * q))
+  (ensures ((pow m (d + r * phi_n)) % n  == (pow m d) % n))
+let lemma_exp_blinding n phi_n p q d m r =
+  if (m = 0 || m % p = 0 || m % q = 0) then
+    lemma_exp_blinding_0 n phi_n p q d m r
+  else lemma_exp_blinding_1 n phi_n p q d m r
+
+val lemma_exp_blinding_bn:
+  #nBits:size_pos -> #pBits:size_pos -> #qBits:size_pos{pBits + qBits < max_size_t} ->
+  #dBits:size_pos -> #mBits:size_pos ->
+  n:bignum nBits{bn_v n > 1} -> phi_n:bignum (pBits+qBits) ->
+  p:bignum pBits{1 < bn_v p /\ bn_v p < bn_v n} -> q:bignum qBits{1 < bn_v q /\ bn_v q < bn_v n} ->
+  d:bignum dBits{0 < bn_v d /\ bn_v d < bn_v n} -> m:bignum mBits{bn_v m < bn_v n} ->
+  r:bignum 64 -> Lemma
+  (requires (bn_v phi_n == (bn_v p - 1) * (bn_v q - 1) /\ bn_v n = bn_v p * bn_v q))
+  (ensures ((pow (bn_v m) (bn_v d + bn_v r * bn_v phi_n)) % bn_v n  == (pow (bn_v m) (bn_v d)) % bn_v n))
+let lemma_exp_blinding_bn #nBits #pBits #qBits #dBits #mBits n phi_n p q d m r =
+  lemma_exp_blinding (bn_v n) (bn_v phi_n) (bn_v p) (bn_v q) (bn_v d) (bn_v m) (bn_v r)
